specs/Spec.GF128.fst
@@ -13,48 +13,51 @@ let elem = felem gf128
 let zero = zero #gf128
 
 (* GCM types and specs *)
-let blocksize : size_nat = 16
-let keysize   : size_nat = 16
-type block = lbytes blocksize
-type tag   = lbytes blocksize
-type key   = lbytes keysize
+inline_for_extraction
+let size_block : size_nat = 16
+inline_for_extraction
+let size_key   : size_nat = 16
 
-let encode (len:size_nat{len <= blocksize}) (w:lbytes len) : Tot elem =
-  let b = create blocksize (u8 0) in
+type block = lbytes size_block
+type tag   = lbytes size_block
+type key   = lbytes size_key
+
+let encode (len:size_nat{len <= size_block}) (w:lbytes len) : Tot elem =
+  let b = create size_block (u8 0) in
   let b = update_slice b 0 len w  in
   to_felem (nat_from_bytes_be b)
 
-let decode (e:elem) : Tot block = nat_to_bytes_be blocksize (from_felem e)
+let decode (e:elem) : Tot block = nat_to_bytes_be size_block (from_felem e)
 
-let update (r:elem ) (len:size_nat{len <= blocksize}) (w:lbytes len) (acc:elem) : Tot elem =
+let update (r:elem ) (len:size_nat{len <= size_block}) (w:lbytes len) (acc:elem) : Tot elem =
     (encode len w `fadd` acc) `fmul` r
 
 val poly: len:size_nat -> text:lbytes len -> r:elem ->  Tot (a:elem)  (decreases len)
 let poly len text r =
-  let blocks = len / blocksize in
-  let rem = len % blocksize in
+  let blocks = len / size_block in
+  let rem = len % size_block in
   let init  : elem = zero in
   let acc   : elem =
     repeati blocks
       (fun i acc  ->
-	let b = slice text (i * blocksize) ((i+1)*blocksize) in
-	update r blocksize b acc)
+	let b = slice text (i * size_block) ((i+1)*size_block) in
+	update r size_block b acc)
       init in
   let acc = if rem = 0 then acc else
     update r rem (slice text (len-rem) len) acc in
   acc
-let finish (a:elem) (s:tag) : Tot tag = decode (a `fadd` (encode blocksize s))
+let finish (a:elem) (s:tag) : Tot tag = decode (a `fadd` (encode size_block s))
 
-let gmul (len:size_nat) (text:lbytes len) (h:lbytes blocksize) : Tot tag  =
-    let r = encode blocksize h in
+let gmul (len:size_nat) (text:lbytes len) (h:lbytes size_block) : Tot tag  =
+    let r = encode size_block h in
     decode (poly len text r)
 
 val gmac:
   len:size_nat ->
   text:lbytes len ->
-  h:lbytes blocksize ->
+  h:lbytes size_block ->
   k:key ->
   Tot tag
 let gmac len text h k =
-  let r = encode blocksize h in
+  let r = encode size_block h in
   finish (poly len text r) k
